adding definitions and lemma statements for new eval_ctx approach

src/simple-proof/proof/Definitions.v
@@ -128,39 +128,22 @@ Definition defs_hasnt(ds: defs)(l: label) := get_def l ds = None.
 (** Typing environment ([G]) *)
 Definition ctx := env typ.
 
-(** ** Evaluation Contexts
-
-The paper defines an evaluation context with the following context-free grammar:
-
-[e ::= [] | let x = [] in t | let x = v in e]
-
-This grammar generates the language characterized by the regular expression:
-
-[ (let x = v in)* []  ]               #<br>#
-[| (let x = v in)* let x = [] in t]
-
-It is more convenient in Coq to represent evaluation contexts following the above
-regular expression.
-
-The sequence of variable-to-value let bindings, [(let x = v in)*],
-is represented as a value environment that maps variables to values: *)
+(** The sequence of variable-to-value let bindings, [(let x = v in)*],
+     is represented as a value environment that maps variables to values: *)
 Definition sto := env val.
 
-(** Now, an evaluation context is either
-    - [e_hole s], where [s] is a (possibly empty) store, which
-      represents [(let x = v in)* []], or
-    - [e_term s t], where [s] is the store and [t] the term to
-      be evaluated next, which represents [(let x = v in)* let x = [] in t]. *)
-Inductive ec : Type :=
-| e_hole : sto -> ec
-| e_term : sto -> trm -> ec.
+(** * Normal Forms
+A normal form is defined in the WadlerFest DOT paper as:
 
-(** A function that retrieves the store from an evaluation context. *)
-Definition ec_sto (e : ec) :=
-  match e with
-  | e_hole s   => s
-  | e_term s t => s
-  end.
+[n ::= x | v | let x = v in n]
+
+This corresponds to an evaluation context of the form
+[(let x = v in)* [ ]] whose hole is filled by a variable [x]
+or value [v]. *)
+
+Inductive normal_form: trm -> Prop :=
+| nf_var: forall x, normal_form (trm_var x)
+| nf_val: forall v, normal_form (trm_val v).
 
 (** * Opening *)
 (** Opening takes a bound variable that is represented with a de Bruijn index [k]
@@ -316,20 +299,6 @@ Inductive lc_sto : sto -> Prop :=
     lc_val v ->
     lc_sto (s & x ~ v).
 
-(** Locally closed evaluation contexts *)
-Inductive lc_ec : ec -> Prop :=
-| lc_ec_hole : forall s,
-    lc_sto s ->
-    lc_ec (e_hole s)
-| lc_ec_term : forall s t,
-    lc_sto s ->
-    (forall x, lc_trm (open_trm x t)) ->
-    lc_ec (e_term s t).
-
-(** Locally closed terms that are decomposed using evaluation contexts *)
-Definition lc_term (e : ec) (t : trm) : Prop :=
-  lc_ec e /\ lc_trm t.
-
 (** * Free variables
       Functions that retrieve the free variables of a symbol. *)
 
@@ -382,13 +351,6 @@ with fv_defs(ds: defs) : vars :=
   | defs_cons tl d   => (fv_defs tl) \u (fv_def d)
   end.
 
-(** Free variables in an evaluation context *)
-Fixpoint fv_ec (e: ec) : vars :=
-  match e with
-  | e_hole s => dom s
-  | e_term s t => dom s \u (fv_trm t)
-  end.
-
 (** Free variables in the range (types) of a context *)
 Definition fv_ctx_types(G: ctx): vars := (fv_in_values (fun T => fv_typ T) G).
 
@@ -407,8 +369,8 @@ Ltac gather_vars :=
   let H := gather_vars_with (fun x : def       => fv_def   x) in
   let I := gather_vars_with (fun x : defs      => fv_defs  x) in
   let J := gather_vars_with (fun x : typ       => fv_typ   x) in
-  let K := gather_vars_with (fun x : ec        => fv_ec    x) in
-  constr:(A \u B \u C \u D \u E \u F \u G \u H \u I \u J \u K).
+  (* let K := gather_vars_with (fun x : ec        => fv_ec    x) in *)
+  constr:(A \u B \u C \u D \u E \u F \u G \u H \u I \u J (* \u K *) ).
 
 Ltac pick_fresh x :=
   let L := gather_vars in (pick_fresh_gen L x).
@@ -442,158 +404,6 @@ Tactic Notation "SSCase" constr(name) := Case_aux SSCase name.
 Tactic Notation "SSSCase" constr(name) := Case_aux SSSCase name.
 Tactic Notation "SSSSCase" constr(name) := Case_aux SSSSCase name.
 Tactic Notation "SSSSSCase" constr(name) := Case_aux SSSSSCase name.
-
-(** * Operational Semantics
-
-The reduction rules in the paper are:
-
-[t |-> t']                 #<br>#
-[――――――――――――――] (Term)  #<br>#
-[e[t] |-> e[t']] #<br># #<br>#
-
-[v = lambda(z: T).t]                                      #<br>#
-[―――――――――――――――――――――――――――――――――――――――――――――――] (Apply) #<br>#
-[let x = v in e[x y] |-> let x = v in e[[y/z] t]] #<br># #<br>#
-
-[v = nu(x: T)...{a = t}...]                             #<br>#
-[―――――――――――――――――――――――――――――――――――――――――] (Project)   #<br>#
-[let x = v in e[x.a] |-> let x = v in e[t]] #<br># #<br>#
-
-[let x = y in t |-> [y/x] t] (Let-Var) #<br># #<br>#
-
-[let x = let y = s in t in y |-> let y = s in let x = t in u] (Let-Let) #<br># #<br>#
-
-We transform the rules by inlining the (Term) rule into all of the other rules:
-
-[v = lambda(z: T).t]                                                #<br>#
-[―――――――――――――――――――――――――――――――――――――――――――――――――――――――――] (Apply) #<br>#
-[e1[let x = v in e2[x y]] |-> e1[let x = v in e2[[y/z] t]]] #<br># #<br>#
-
-[v = nu(x: T)...{a = t}...]                                           #<br>#
-[―――――――――――――――――――――――――――――――――――――――――――――――――――――――――] (Project) #<br>#
-[e1[let x = v in e2[x.a]] |-> e1[let x = v in e2[t]]] #<br># #<br>#
-
-[e[let x = y in t] |-> e[[y/x] t]] (Let-Var) #<br># #<br>#
-
-[e[let x = let y = s in t in u] |-> e[let y = s in let x = t in u]] (Let-Let) #<br># #<br>#
-
-We then note that in the Apply and Project rules,
-[e1[let x = v in e2[ ]]]
-is itself a larger evaluation context. We simplify this evaluation context
-into just [e[ ]].
-
-Additionally, we define a binds relation [e(x) = v] which determines
-whether the evaluation context [e] contains the subterm [let x = v in e2]:
-
-[e = e1[let x = v in e2[ ]]] #<br>#
-[――――――――――――――――――――――――――] #<br>#
-[e(x) = v] #<br># #<br>#
-
-The (Apply) and (Project) reduction rules become:
-
-[e(x) = lambda(z: T).t]         #<br>#
-[―――――――――――――――――――――] (Apply) #<br>#
-[e[x y] |-> e[[y/z] t]] #<br># #<br>#
-
-[e(x) = nu(x: T)...{a = t}...]           #<br>#
-[――――――――――――――――――――――――――――] (Project) #<br>#
-[e[x.a] |-> e[t]] #<br># #<br>#
-
-In general, there may be multiple decompositions of a term into an evaluation context
-and a subterm. For example, the term
-
-[let x = v1 in let y = v2 in x y]
-
-decomposes in three ways:
-
-[[let x = v1 in let y = v2 in x y]]
-
-[let x = v1 in [let y = v2 in x y]]
-
-[let x = v1 in let y = v2 in [x y]]
-
-However, the reduction rules cannot apply to any of the decompositions except the
-last one, because none of the reduction rules match the syntactic pattern
-
-[e[let x = v in t]]
-
-Therefore, the only decomposition to which a reduction rule can possibly apply
-is the maximal one, where all prefixes of the form
-
-[let x = v in]
-
-have been shifted into the evaluation context.
-
-In the proof, we represent terms in this maximally decomposed way, in the form
-of a pair [(e, t)] of an evaluation context and a term.
-
-A term of the form
-
-[let x = t in u]
-
-can be decomposed into evaluation contexts in two ways:
-
-[[let x = t in u]]  (1)
-
-[let x = [t] in u]  (2)
-
-Similarly, a term of the form
-
-[let x = v in u]
-
-can be decomposed into evaluation contexts in three ways:
-
-[[let x = v in u]]  (3)
-
-[let x = [v] in u]  (4)
-
-[let x = v in [u]]  (5)
-
-Of these different decompositions of the same two terms, the reduction
-rules can apply only to decompositions (2) and (5).
-
-We add congruence reduction rules to reduce the decomposition (1) to
-decomposition (2) and decompositions (3) and (4) to decomposition (5).
-
-[e[let x = t in u] |-> e[let x = [t] in u]]
-(Congruence-Let) #<br># #<br>#
-
-[e[let x = [v] in u] |-> e[let x = v in [u]]]
-(Congruence-Val) #<br># #<br>#
-
-Rule (Congruence-Let) reduces (1) to (2). It also reduces (3) to (4).
-Rule (Congruence-Val) then further reduces (4) to (5). *)
-
-Reserved Notation "e1 '/' t1 '|->' e2 '/' t2" (at level 40, e2 at level 39).
-
-Inductive red : ec -> trm -> ec -> trm -> Prop :=
-(** [e(x) = lambda(T)t]  #<br>#
-    [――――――――――――]  #<br>#
-    [e | x y |-> e | t^y]  *)
-| red_apply : forall x y e T t,
-    binds x (val_lambda T t) (ec_sto e) ->
-    e / trm_app (avar_f x) (avar_f y) |-> e / open_trm y t
-(** [e(x) = nu(T)...{a = t}...]  #<br>#
-    [――――――――――――――――――――――――]  #<br>#
-    [e | x.a |-> e | t]  *)
-| red_project : forall x a e T ds t,
-    binds x (val_new T ds) (ec_sto e) ->
-    defs_has (open_defs x ds) (def_trm a t) ->
-    e / trm_sel (avar_f x) a |-> e / t
-(** [e[let x = [ ] in t] | y |-> e[ ] | t^y] *)
-| red_let_var : forall x t s,
-    e_term s t / trm_var (avar_f x) |-> e_hole s / open_trm x t
-(** [e[let x = [ ] in t1] | let t2 in t3 |-> e[let x = [ ] in let t3 in t1] | t2] *)
-| red_let_let : forall s t1 t2 t3,
-    e_term s t1 / trm_let t2 t3 |-> e_term s (trm_let t3 t1) / t2
-(** [e[ ] | let x = t in u |-> e[let x = [ ] in u] | t] *)
-| red_congruence_let : forall s t u,
-    e_hole s / trm_let t u |-> e_term s u / t
-(** [e[let x = [ ] in t] | v |-> e[let x = v in [ ]] | t^x] *)
-| red_congruence_val: forall s x v t,
-    x # s ->
-    e_term s t / trm_val v |-> e_hole (s & (x ~ v)) / open_trm x t
-where "t1 '/' st1 '|->' t2 '/' st2" := (red t1 st1 t2 st2).
 
 (** * Typing Rules *)
 
@@ -1302,36 +1112,14 @@ Inductive inert : ctx -> Prop :=
       x # G ->
       inert (G & x ~ T).
 
-(** ** Typing of Evaluation Contexts *)
-
-(** We define a typing relation for pairs [e] and [t] of an evaluation context and a term
-    in an empty context.
-
-    The term [e[t]] has type T in an empty context if and only if [G] is inert,
-    [G] corresponds to the store of [e], and the term [e[t]] has type [T] in typing context
-    [G] according to the general typing relation for terms . *)
-Inductive ty_ec_trm: ctx -> ec -> trm -> typ -> Prop :=
-| ty_e_hole : forall G s t T,
-    inert G ->
-    G ~~ s ->
-    G |- t : T ->
-    ty_ec_trm G (e_hole s) t T
-| ty_e_term : forall L G s u t T U,
-    inert G ->
-    G ~~ s ->
-    G |- t : T ->
-    (forall x, x \notin L -> G & x ~ T |- (open_trm x u) : U) ->
-    ty_ec_trm G (e_term s u) t U.
-
-
 (** * Infrastructure *)
 
 Hint Constructors
-     inert_typ inert wf_sto record_has
+     normal_form inert_typ inert record_has
      ty_trm ty_def ty_defs subtyp ty_trm_p
      ty_trm_t subtyp_t ty_var_inv ty_val_inv
      lc_var lc_typ lc_dec lc_trm lc_val
-     lc_dec lc_defs lc_sto lc_ec.
+     lc_dec lc_defs lc_sto.
 
 (** ** Mutual Induction Principles *)
 
