src/simple-proof/proof/Safety.v
@@ -6,269 +6,71 @@
 
 Set Implicit Arguments.
 
-Require Import LibLN.
 Require Import Coq.Program.Equality.
+Require Import LibLN.
 Require Import Definitions.
-Require Import Weakening.
-Require Import Narrowing.
-Require Import Helper_lemmas.
-Require Import Precise_types.
-Require Import Substitution.
-Require Import Canonical_forms.
+Require Import Operational_semantics.
+Require Import Weakening Narrowing Helper_lemmas Precise_types Substitution Canonical_forms.
 
-(** * Normal Forms
-A normal form is defined in the WadlerFest DOT paper as:
+(** Reduction in an empty context *)
+Notation "t '|->' u" := (empty [t |-> u]) (at level 50).
 
-[n ::= x | v | let x = v in n]
-
-This corresponds to an evaluation context of the form
-[(let x = v in)* [ ]] whose hole is filled by a variable [x]
-or value [v]. *)
-
-Inductive normal_form_trm: trm -> Prop :=
-| nf_var: forall x, normal_form_trm (trm_var x)
-| nf_val: forall v, normal_form_trm (trm_val v).
-
-Definition normal_form (e : ec) (t : trm) : Prop :=
-  match e with
-  | e_hole _   => normal_form_trm t
-  | e_term _ _ => False
-  end.
-
-Hint Unfold normal_form.
-Hint Constructors normal_form_trm.
-
-Inductive closed_ec_typing : ec -> trm -> typ -> Prop :=
-| cet: forall G e t T, ty_ec_trm G e t T ->
-  closed_ec_typing e t T.
-
-Notation "'|-' e '[' t ']:' T" := (closed_ec_typing e t T) (at level 40, t at level 59).
-
-(** If the term [(let x = v in)* let x = [t] in u] represented by an
-    evaluation context is locally closed, so is the term
-    [(let x = v in)* [t]]. *)
-Lemma lc_term_to_hole: forall s u t,
-    lc_term (e_term s u) t ->
-    lc_term (e_hole s) t.
-Proof.
-  intros. inversions H. inversions H0. repeat constructor~.
-Qed.
+(** Typing in an empty context *)
+Notation "'|-' t ':' T" := (empty |- t: T) (at level 40, t at level 59).
 
 (** * Progress *)
 
-(** If [(let x = v in)* let y = [t] in u]
-    reduces to [(let x = v in)* let y = [t'] in u],
-    then [(let x = v in)* [t]]
-    reduces to [(let x = v in)* [t']].
-
-    This lemma is used to reduce cases involving [let y = [t] in u]
-    into simpler cases involving [[t]]. *)
-Lemma red_term_to_hole: forall s u t t',
-    e_term s u / t |-> e_term s u / t' ->
-    e_hole s / t |-> e_hole s / t'.
+(** todo: doc*)
+Lemma progress_ec: forall G e t T,
+    G |- e[t]: T ->
+    (normal_form t \/ exists t', e[t |-> t']).
 Proof.
-  intros. dependent induction H.
-  - eapply red_apply; eauto.
-  - eapply red_project; eauto.
-  - induction u; inversions x.
-    eapply IHu2; eauto.
+  destruct 1 as [* Hwf Ht]. induction Ht; eauto.
+  - Case "ty_all_elim". admit.
+  - Case "ty_new_elim". admit.
+  - Case "ty_let". admit.
 Qed.
 
+
 (** ** Progress Theorem
-    If [|- e[t] : T], then either [e[t]] is a normal form,
-    or [e[t]] reduces to some [e'[t']]. *)
-Lemma progress: forall e t T,
-    |- e[t]: T ->
-    (normal_form e t \/ exists e' t', e / t |-> e' / t').
+    If [|- t : T], then either [t] is a normal form,
+    or [t]] reduces to some [t']. *)
+Theorem progress: forall t T,
+    |- t: T ->
+    normal_form t \/ (exists t', t |-> t').
 Proof.
-  introv Ht. destruct Ht as [* Ht]. destruct e; inversions Ht.
-  - rename H0 into Hi. rename H3 into Ht. rename H1 into Hwf.
-    dependent induction Ht; try solve [left; auto].
-    * destruct (canonical_forms_fun Hi Hwf Ht1) as [L [T' [t [Bis [Hsub Hty]]]]].
-      right. repeat eexists. apply* red_apply.
-    * destruct (canonical_forms_obj Hi Hwf Ht) as [S [ds [t [Bis [Has Ty]]]]].
-      right. repeat eexists. apply* red_project.
-    * right. exists (e_term s u) t.
-      apply red_congruence_let.
-    * specialize (IHHt Hi) as [IH | [t' [s' Hred]]].
-      + assumption.
-      + left. assumption.
-      + right. exists t' s'. assumption.
-  - clear H7.
-    rename H1 into Hin. rename H2 into Hwf. rename H4 into Ht.
-    dependent induction Ht; right.
-    * repeat eexists; apply red_let_var.
-    * pick_fresh x. repeat eexists; apply red_congruence_val with (x:=x); auto.
-    * destruct (canonical_forms_fun Hin Hwf Ht1) as [L' [T' [t [Bis [Hsub Hty]]]]].
-      repeat eexists. apply* red_apply.
-    * pick_fresh x. repeat eexists; apply red_congruence_val with (x:=x); auto.
-    * destruct (canonical_forms_obj Hin Hwf Ht) as [S [ds [t [Bis [Has Ty]]]]].
-      repeat eexists. apply* red_project.
-    * repeat eexists; apply red_let_let.
-    * repeat eexists; apply red_let_var.
-    * repeat eexists; apply red_let_var.
-    * repeat eexists; apply red_let_var.
-    * specialize (IHHt Hin) as [IH | [t' [s' Hred]]]; eauto.
-      inversion IH.
+  introv Ht. assert (empty |- empty[t]: T) as He by (repeat constructor*).
+  apply* progress_ec.
 Qed.
 
 (** * Preservation *)
 
-(** Reduction preserves local closure. *)
-Lemma red_preserves_lc :
-  forall e t e' t',
-    e / t |-> e' / t' ->
-    lc_term e t ->
-    lc_term e' t'.
+Lemma preservation_ec: forall G e t t' T,
+  G |- e[t]: T ->
+  e[t |-> t'] ->
+  G |- e[t']: T.
 Proof.
-  intros.
-  destruct H0.
-  dependent induction H; try solve [inversions H1; inversions H0; split*].
-  - pose proof (lc_ec_sto_inv H0).
-    pose proof (lc_ec_sto_binds_inv H0 H).
-    inversions H3. split~.
-  - pose proof (lc_ec_sto_binds_inv H1 H). inversions H3.
-    pose proof (lc_defs_has (H7 x) H0). inversions H3. split~.
-  - inversions H0. inversions H1.
-    split; auto. eapply lc_ec_term; auto.
-    intros x. unfold open_trm.
-    simpl. eapply lc_trm_let; auto.
-    intros x0. unfold open_trm.
-    rewrite~ (proj1 (open_comm_trm_val_def_defs x0 x)).
-    rewrite~ lc_opening.
-Qed.
-
-(** Special case of type preservation for evaluation contexts of the
-    form [(let x=v in)* [ ]].
-
-    If [e] and [t] are locally closed, [|- e[t]: T],
-    and [e[t] |-> e'[t']], then [|- e'[t']: T]. *)
-Lemma red_preserves_type_hole: forall G s t e' t' T,
-    lc_term (e_hole s) t ->
-    e_hole s / t |-> e' / t' ->
-    ty_ec_trm G (e_hole s) t T ->
-    exists G', ty_ec_trm (G & G') e' t' T.
-Proof.
-  introv Hlc Hred Ht.
-  inversions Ht.
-  rename H0 into Hin. rename H1 into Hwf. rename H3 into Ht.
-  lets Hlc': (red_preserves_lc Hred Hlc).
-  dependent induction Ht; try solve [inversion Hred].
-  - destruct (canonical_forms_fun Hin Hwf Ht1) as [L [T' [t [Bis [Hsub Hty]]]]].
-    inversions Hred.
-    apply (binds_func H4) in Bis. inversions Bis.
-    exists (@empty typ). rewrite concat_empty_r.
-    pick_fresh y. assert (y \notin L) as FrL by auto. specialize (Hty y FrL).
-    constructor*. rewrite subst_intro_typ with (x:=y); auto.
-    rewrite subst_intro_trm with (x:=y); auto.
-    eapply subst_ty_trm; eauto. rewrite~ subst_fresh_typ.
-  - destruct (canonical_forms_obj Hin Hwf Ht) as [S [ds [t [Bis [Has Ty]]]]].
-    inversions Hred.
-    apply (binds_func H2) in Bis. inversions Bis.
-    exists (@empty typ). rewrite concat_empty_r.
-    rewrite <- (defs_has_inv Has H5). constructor*.
-  - inversions Hred.
-    exists (@empty typ). rewrite concat_empty_r.
-    eapply ty_e_term; eauto.
-  - specialize (IHHt Hlc Hred Hin Hwf Hlc') as [G' IHHt].
-    exists G'. inversions IHHt.
-    + eapply ty_e_hole; auto.
-      apply weaken_subtyp with (G2:=G') in H; eauto.
-    + apply_fresh ty_e_term as z; eauto; intros. assert (z \notin L) by auto.
-      specialize (H3 z H4).
-      apply weaken_subtyp with (G2:=(G' & z ~ T0)) in H; rewrite concat_assoc in *; eauto.
-Qed.
-
-(** Type Preservation:
-    If [e] and [t] are locally closed, [|- e[t]: T], and [e[t] |-> e'[t']],
-    then [|- e'[t']: T]. *)
-Lemma red_preserves_type: forall G e t e' t' T,
-    lc_term e t ->
-    e / t |-> e' / t' ->
-    ty_ec_trm G e t T ->
-    exists G', ty_ec_trm (G & G') e' t' T.
-Proof.
-  introv Hlc Hred Ht.
-  inversions Ht; rename H into Hin; rename H0 into Hwf; rename H1 into Ht.
-  inversion Hlc as [Hlc_ec Hlc_trm].
-  apply* red_preserves_type_hole. constructor~.
-  destruct t.
-  - inversions Hred.
-    pick_fresh y.
-    exists (@empty typ). rewrite concat_empty_r.
-    apply ty_e_hole; auto.
-    rewrite subst_intro_trm with (x:=y); auto.
-    rewrite <- subst_fresh_typ with (x:=y) (y:=x); auto.
-    eapply subst_ty_trm; auto. rewrite~ subst_fresh_typ.
-  - inversions Hred.
-    pose proof (wf_sto_notin_dom Hwf H5).
-    pose proof (val_typing Ht) as [V [Hv Hs]].
-    pick_fresh y. assert (y \notin L) by auto.
-    specialize (H2 y H0).
-    exists (x ~ V).
-    apply ty_e_hole.
-    * constructor~. eapply precise_inert_typ; eauto.
-    * constructor~.
-      apply (precise_to_general Hv).
-    * rewrite subst_intro_trm with (x:=y); auto.
-      rewrite <- subst_fresh_typ with (x:=y) (y:=x); auto.
-      eapply subst_ty_trm; auto.
-      { eapply weaken_rules; eauto. }
-      { apply~ fv_ctx_types_push. }
-      {
-        rewrite~ subst_fresh_typ.
-        pose proof (ty_var (binds_tail x V G)).
-        apply (ty_sub H1). apply (weaken_subtyp Hs); eauto.
-      }
-  - inversion Hred. rewrite <- H4 in Hred. apply red_term_to_hole in Hred. subst.
-    apply lc_term_to_hole in Hlc.
-    pose proof (red_preserves_type_hole Hlc Hred (ty_e_hole Hin Hwf Ht)) as [G' Ht'].
-    inversions Ht'. exists G'.
-    eapply ty_e_term with (L:=L \u (dom G) \u (dom G')); eauto. intros.
-    assert (x0 \notin L) by auto.
-    specialize (H2 x0 H4).
-    eapply (proj41 weaken_rules); eauto.
-  - inversion Hred. rewrite <- H1 in Hred.
-    apply red_term_to_hole in Hred. subst.
-    apply lc_term_to_hole in Hlc.
-    pose proof (red_preserves_type_hole Hlc Hred (ty_e_hole Hin Hwf Ht)) as [G' Ht'].
-    inversions Ht'. exists G'.
-    eapply ty_e_term with (L:=L \u (dom G) \u (dom G')); eauto. intros.
-    eapply (proj41 weaken_rules); eauto.
-  - inversions Hred.
-    exists (@empty typ). rewrite concat_empty_r.
-    gen L.
-    dependent induction Ht; intros.
-    + eapply ty_e_term with (L:=L \u (dom G)); eauto. intros.
-      assert (x \notin L) by auto.
-      unfold open_trm. simpl. specialize (H x H3).
-      apply_fresh ty_let as z; eauto.
-      unfold open_trm.
-      rewrite~ (proj41 (open_comm_trm_val_def_defs z x)).
-      inversion Hlc as [Hlc_ec Hlc_trm].
-      inversions Hlc_ec. specialize (H7 z).
-      apply (lc_opening 1 x) in H7. unfold open_trm in H7. rewrite H7.
-      assert (z \notin L0) by auto.
-      specialize (H2 z H4).
-      eapply weaken_rules; eauto.
-    + eapply IHHt with (L:=L \u (dom G)); auto. intros.
-      assert (x \notin L) by auto.
-      specialize (H2 x H1).
-      eapply narrow_typing; eauto. apply~ subenv_last.
+  destruct 1 as [* Hwf Ht]. induction Ht.
+  - Case "ty_var". admit.
+  - Case "ty_all_intro". admit.
+  - Case "ty_all_elim". admit.
+  - Case "ty_new_intro". admit.
+  - Case "ty_new_elim". admit.
+  - Case "tylet". admit.
+  - Case "ty_rec_intro". admit.
+  - Case "ty_rec_elim". admit.
+  - Case "ty_and_intro". admit.
+  - Case "ty_sub". admit.
 Qed.
 
 (** ** Preservation Theorem
-    Reduction preserves both local closure and the type of the term being reduced.
-
-    If [e] and [t] are locally closed, [|- e[t]: T], and [e[t] |-> e'[t']], then
-    [e'] and [t'] are locally closed and [|- e'[t']: T]. *)
-Lemma preservation: forall e t e' t' T,
-    lc_term e t ->
-    e / t |-> e' / t' ->
-    |- e [t]: T ->
-    lc_term e' t' /\ |- e' [t']: T.
+    If [|- t : T] and [t |-> t'], then [|- t': T]. *)
+Theorem preservation: forall (t t' : trm) T,
+  |- t: T ->
+  t |-> t' ->
+  |- t' : T.
 Proof.
-  introv Hl Hr Ht. split. apply* red_preserves_lc. destruct Ht.
-  destruct (red_preserves_type Hl Hr H) as [G' Hty].
-  econstructor. eauto.
+  introv Ht Hr.
+  assert (empty |- empty[t]: T) as He by (repeat constructor*).
+  destruct* (preservation_ec He Hr).
 Qed.
