src/simple-proof/proof/Operational_semantics.v
@@ -1,0 +1,55 @@
+Set Implicit Arguments.
+
+Require Import LibLN.
+Require Import Definitions.
+
+(** * Operational Semantics *)
+
+Reserved Notation "e '[' t1 '|->' t2 ']'" (at level 60, t1 at level 39).
+
+Inductive red : sto -> trm -> trm -> Prop :=
+(** [e(x) = lambda(T)t]    #<br>#
+    ―――――――――――――――――――――  #<br>#
+    [e [x y] |-> e [t^y] ]  *)
+| red_apply : forall x y e T t,
+    binds x (val_lambda T t) e ->
+    e [ trm_app (avar_f x) (avar_f y) |-> open_trm y t ]
+(** [e(x) = nu(T)...{a = t}...]  #<br>#
+    ―――――――――――――――――――――――――――  #<br>#
+    [e[ x.a] |-> e[t]]  *)
+| red_project : forall x a e T ds t,
+    binds x (val_new T ds) e ->
+    defs_has (open_defs x ds) (def_trm a t) ->
+    e [ trm_sel (avar_f x) a |-> t ]
+(** [e[let x = y in t] |-> e[t^y]] *)
+| red_let_var : forall y t e,
+    e [ trm_let (trm_var (avar_f y)) t |-> open_trm y t ]
+(** [e[let x = (let y = s in t) in u] |-> e[let y = s in let x = t in u]] *)
+| red_let_let : forall s t u e,
+    e [ trm_let (trm_let s t) u |-> trm_let s (trm_let t u) ]
+(** [e[t] |-> e[t']]                            #<br>#
+    ――――――――――――――――――――――――――――――――――――――――――― #<br>#
+    e[let x = t in u] |-> e[let x = t' in u]]     *)
+| red_let_trm : forall e t t' u,
+    e [ t |-> t' ] ->
+    e [ trm_let t u |-> trm_let t' u ]
+(** [e[t] |-> e[t']]                            #<br>#
+    ――――――――――――――――――――――――――――――――――――――――――― #<br>#
+    e[let x = v in t] |-> e[let x = v in t']]     *)
+| red_let_val: forall e t t' v,
+    e [ t  |-> t' ] ->
+    e [ trm_let (trm_val v) t |-> trm_let (trm_val v) t' ]
+where "e [ t |-> t' ]" := (red e t t').
+
+(** ** Typing of Evaluation Contexts *)
+
+(** We define a typing relation for pairs [e] and [t] of an evaluation context and a term. *)
+
+Reserved Notation "G '|-' e '[' t ']:' T" (at level 40, e at level 59).
+
+Inductive ty_ec : ctx -> sto -> trm -> typ -> Prop :=
+| ty_ec_c : forall G e t T,
+    G ~~ e ->
+    G |- t : T ->
+    G |- e[t]: T
+ where "G '|-' e '[' t ']:' T" := (ty_ec G e t T).
